src/ReactorModel/Execution/Determinism.lean
@@ -8,6 +8,10 @@ def List.lastSome? (f : α → Option β) : List α → Option β
     | some b => some b
     | none   => f a
 
+theorem List.lastSome?_eq_some_iff {l : List α} : 
+  (∃ b, l.lastSome? f = some b) ↔ (∃ b a, a ∈ l ∧ (f a) = some b) := 
+  sorry
+
 -- This file defines (and proves) determinism for the reactor model.
 -- Determinism can be understood in multiple ways.
 -- Primarily, we say the execution is deterministic if there is always at most one timed
@@ -137,11 +141,11 @@ theorem ChangeListStep.indep_comm_ids {s s₁ s₂ s₁₂ s₂₁ : State} {rcn
   sorry
 -/
 
-theorem ChangeListStep.preserves_ctx : (s₁ -[cs]→* s₂) → s₁.ctx = s₂.ctx 
+theorem ChangeListStep.preserves_ctx : (s₁ -[rcn:cs]→* s₂) → s₁.ctx = s₂.ctx 
   | .nil .. => rfl
   | .cons h₁₂ h₂₃ => h₁₂.preserves_ctx.trans h₂₃.preserves_ctx
 
-theorem ChangeListStep.preserves_rcns {i : ID} : (s₁ -[cs]→* s₂) → (s₁.rtr.obj? .rcn i = s₂.rtr.obj? .rcn i)
+theorem ChangeListStep.preserves_rcns {i : ID} : (s₁ -[rcn:cs]→* s₂) → (s₁.rtr.obj? .rcn i = s₂.rtr.obj? .rcn i)
   | .nil .. => rfl
   | .cons h₁₂ h₂₃ => h₁₂.preserves_rcns.trans h₂₃.preserves_rcns
 
@@ -249,12 +253,30 @@ theorem ChangeStep.preserves_unchanged_state {i : ID} :
     contradiction
   case' action h, port h => exact Reactor.Update.preserves_ne_cmp_or_id h (.inl $ by simp) (by simp) (by simp)
 
-theorem ChangeListStep.preserves_Equiv : (s₁ -[cs]→* s₂) → s₁.rtr ≈ s₂.rtr
+theorem ChangeStep.preserves_port_role {i : ID} :
+  (s₁ -[rcn:c]→ s₂) → (s₁.rtr.obj? .prt i = some p) → (∃ v, s₂.rtr.obj? .prt i = some ⟨p.role, v⟩) := by
+  intro hs ho
+  cases hs
+  case port j v h =>
+    have ⟨_, ho', hv⟩ := h.change'
+    by_cases hi : i = j
+    case pos =>
+      exists v
+      rw [hi] at ho ⊢
+      simp [ho.symm.trans ho' |> Option.some_inj.mp, hv]
+    case neg =>
+      exists p.val
+      simp [←h.preserves_ne_cmp_or_id (cmp' := .prt) (i' := i) (by simp [hi]) (by simp) (by simp), ho]
+  all_goals exists p.val
+  case' state h, action h => simp [←h.preserves_ne_cmp_or_id (cmp' := .prt) (i' := i) (by simp) (by simp) (by simp), ho]
+  all_goals exact ho
+  
+theorem ChangeListStep.preserves_Equiv : (s₁ -[rcn:cs]→* s₂) → s₁.rtr ≈ s₂.rtr
   | nil .. => .refl
   | cons h hi => h.preserves_Equiv.trans hi.preserves_Equiv
 
 theorem ChangeListStep.preserves_unchanged_ports {i : ID} :
-  (s₁ -[cs]→* s₂) → (∀ v, .port i v ∉ cs) → (s₁.rtr.obj? .prt i = s₂.rtr.obj? .prt i)
+  (s₁ -[rcn:cs]→* s₂) → (∀ v, .port i v ∉ cs) → (s₁.rtr.obj? .prt i = s₂.rtr.obj? .prt i)
   | nil ..,    _ => rfl
   | cons h hi, hc => by
     refine (h.preserves_unchanged_port ?_).trans (hi.preserves_unchanged_ports ?_) <;> (
@@ -264,7 +286,7 @@ theorem ChangeListStep.preserves_unchanged_ports {i : ID} :
     )
 
 theorem ChangeListStep.preserves_unchanged_actions {i : ID} :
-  (s₁ -[cs]→* s₂) → (∀ t v, .action i t v ∉ cs) → (s₁.rtr.obj? .act i = s₂.rtr.obj? .act i)
+  (s₁ -[rcn:cs]→* s₂) → (∀ t v, .action i t v ∉ cs) → (s₁.rtr.obj? .act i = s₂.rtr.obj? .act i)
   | nil ..,    _ => rfl
   | cons h hi, hc => by
     refine (h.preserves_unchanged_action ?_).trans (hi.preserves_unchanged_actions ?_) <;> (
@@ -274,7 +296,7 @@ theorem ChangeListStep.preserves_unchanged_actions {i : ID} :
     )
 
 theorem ChangeListStep.preserves_unchanged_state {i : ID} :
-  (s₁ -[cs]→* s₂) → (∀ v, .state i v ∉ cs) → (s₁.rtr.obj? .stv i = s₂.rtr.obj? .stv i)
+  (s₁ -[rcn:cs]→* s₂) → (∀ v, .state i v ∉ cs) → (s₁.rtr.obj? .stv i = s₂.rtr.obj? .stv i)
   | nil ..,    _ => rfl
   | cons h hi, hc => by
     refine (h.preserves_unchanged_state ?_).trans (hi.preserves_unchanged_state ?_) <;> (
@@ -283,9 +305,10 @@ theorem ChangeListStep.preserves_unchanged_state {i : ID} :
       assumption
     )
 
-theorem ChangeListStep.preserves_port_role :
-  (s₁ -[rcn:cs]→* s₂) → (s₁.rtr.obj? .prt i = some p) → (∃ v, s₂.rtr.obj? .prt i = some ⟨p.role, v⟩) := by
-  sorry
+theorem ChangeListStep.preserves_port_role {i : ID} :
+  (s₁ -[rcn:cs]→* s₂) → (s₁.rtr.obj? .prt i = some p) → (∃ v, s₂.rtr.obj? .prt i = some ⟨p.role, v⟩)
+  | nil ..,     ho => ⟨_, ho⟩
+  | cons hd tl, ho => by simp [tl.preserves_port_role (hd.preserves_port_role ho).choose_spec]
 
 theorem ChangeListStep.last_state_value :
   (s₁ -[rcn:cs]→* s₂) → (cs.lastSome? (·.stateValue? i) = some v) → (s₂.rtr.obj? .stv i = some v) := by
@@ -295,7 +318,13 @@ theorem ChangeListStep.last_state_value :
 theorem ChangeListStep.lastSome?_none_preserves_state_value :
   (s₁ -[rcn:cs]→* s₂) → (cs.lastSome? (·.stateValue? i) = none) → (s₁.rtr.obj? .stv i = s₂.rtr.obj? .stv i) := by
   intro hs hl 
-  sorry
+  have h := (mt List.lastSome?_eq_some_iff.mpr) (Option.eq_none_iff_forall_not_mem.mp hl |> not_exists_of_forall_not)
+  exact hs.preserves_unchanged_state (i := i) (by
+    intro v hn
+    simp at h
+    specialize h v (.state i v) hn
+    simp [Change.stateValue?] at h
+  )
 
 theorem ChangeListStep.last_port_value :
   (s₁ -[rcn:cs]→* s₂) → (cs.lastSome? (·.portValue? i) = some v) → (∃ r, s₂.rtr.obj? .prt i = some ⟨r, v⟩) := by
@@ -305,7 +334,13 @@ theorem ChangeListStep.last_port_value :
 theorem ChangeListStep.lastSome?_none_preserves_port_value :
   (s₁ -[rcn:cs]→* s₂) → (cs.lastSome? (·.portValue? i) = none) → (s₁.rtr.obj? .prt i = s₂.rtr.obj? .prt i) := by
   intro hs hl 
-  sorry
+  have h := (mt List.lastSome?_eq_some_iff.mpr) (Option.eq_none_iff_forall_not_mem.mp hl |> not_exists_of_forall_not)
+  exact hs.preserves_unchanged_ports (i := i) (by
+    intro v hn
+    simp at h
+    specialize h v (.port i v) hn
+    simp [Change.portValue?] at h
+  )
 
 theorem ChangeListStep.equiv_changes_eq_result :
   (s -[rcn₁:cs₁]→* s₁) → (s -[rcn₂:cs₂]→* s₂) → (cs₁ ⋈ cs₂) → s₁ = s₂ := by
@@ -420,17 +455,17 @@ theorem InstStep.self_currentProcessedRcns :
 theorem InstStep.preserves_nondep_ports : 
   (s₁ ⇓ᵢ[i] s₂) → (s₁.rtr.obj? .rcn i = some rcn) → (p ∉ rcn.deps .out) → (s₁.rtr.obj? .prt p = s₂.rtr.obj? .prt p)
   | skipReaction ..,        _,  _ => rfl
-  | execReaction _ _ ho hs, hr, hd => hs.preserves_unchanged_ports (s₁.rcnOutput_port_dep_only · (by simp [ho]; sorry /-This is a List.map id-/) hr hd)
+  | execReaction _ _ ho hs, hr, hd => hs.preserves_unchanged_ports (s₁.rcnOutput_port_dep_only · ho hr hd)
 
 theorem InstStep.preserves_nondep_actions : 
   (s₁ ⇓ᵢ[i] s₂) → (s₁.rtr.obj? .rcn i = some rcn) → (a ∉ rcn.deps .out) → (s₁.rtr.obj? .act a = s₂.rtr.obj? .act a)
   | skipReaction ..,        _,  _ => rfl
-  | execReaction _ _ ho hs, hr, hd => hs.preserves_unchanged_actions (s₁.rcnOutput_action_dep_only · · (by simp [ho]; sorry /-This is a List.map id-/) hr hd)
+  | execReaction _ _ ho hs, hr, hd => hs.preserves_unchanged_actions (s₁.rcnOutput_action_dep_only · · ho hr hd)
 
 theorem InstStep.pure_preserves_state {j : ID} : 
   (s₁ ⇓ᵢ[i] s₂) → (s₁.rtr.obj? .rcn i = some rcn) → (rcn.isPure) → (s₁.rtr.obj? .stv j = s₂.rtr.obj? .stv j)
   | skipReaction ..,    _,  _ => rfl
-  | execReaction _ _ ho hs, hr, hp => hs.preserves_unchanged_state (s₁.rcnOutput_pure · (by simp [ho]; sorry /-This is a List.map id-/) hr hp)
+  | execReaction _ _ ho hs, hr, hp => hs.preserves_unchanged_state (s₁.rcnOutput_pure · ho hr hp)
 
 -- Note: We can't express the result as `∀ x, c₁.obj? .stv x = c₂.obj? .stv x`,
 --       as `c₁`/`c₂` might contain `c` as a (transitively) nested reactor. 
@@ -443,7 +478,7 @@ theorem InstStep.preserves_external_state :
     apply hs.preserves_Equiv.nest' hc₁ hc₂ |>.obj?_ext (cmp := .stv)
     intro x hx
     have hm := Reactor.local_mem_exclusive hc₁ (Reactor.con?_to_rtr_obj? hc) hi.symm hx
-    have hu := hs.preserves_unchanged_state (s₁.rcnOutput_state_local · (by simp [ho]; sorry /-This is a List.map id-/) hc hm)
+    have hu := hs.preserves_unchanged_state (s₁.rcnOutput_state_local · ho hc hm)
     exact hs.preserves_Equiv.eq_obj?_nest hu hc₁ hc₂
 
 theorem InstStep.acyclic_deps : (s₁ ⇓ᵢ[rcn] s₂) → (rcn >[s₁.rtr]< rcn) :=
